Mica.lean
@@ -5,3 +5,4 @@ import Mica.TinyML
 import Mica.Verifier
 import Mica.SeparationLogic
 import Mica.Frontend
+import Mica.Stdlib
